format-version: 1.2
data-version: memon/releases/2024-12-12/memon-base.owl
idspace: cito http://purl.org/spar/cito/ 
idspace: dce http://purl.org/dc/elements/1.1/ 
idspace: dcterms http://purl.org/dc/terms/ 
idspace: foaf http://xmlns.com/foaf/0.1/ 
idspace: oboInOwl http://www.geneontology.org/formats/oboInOwl# 
idspace: skos http://www.w3.org/2004/02/skos/core# 
idspace: swrla http://swrl.stanford.edu/ontologies/3.3/swrla.owl# 
ontology: memon/memon-base
property_value: dce:type IAO:8000001
property_value: dcterms:description "An ontology about cell membranes and their models" xsd:string
property_value: dcterms:license https://creativecommons.org/publicdomain/zero/1.0/
property_value: dcterms:title "Membrane Ontology" xsd:string
property_value: owl:versionInfo "2024-12-12" xsd:string

[Term]
id: MEMON:0000001
name: experimental membrane model
def: "A membrane model that is used in experiments." []
is_a: MEMON:0000008 ! membrane model
relationship: RO:0002180 MEMON:0000004 ! membrane model component
property_value: dce:creator "Dominik Martinát" xsd:string
property_value: dce:date "2024-12-08T15:48:12Z" xsd:dateTime

[Term]
id: MEMON:0000002
name: artificial lipid membrane
def: "An experimental membrane model that is prepared from lipids." []
comment: For example membrane consisting of DOPC.
is_a: MEMON:0000001 ! experimental membrane model
property_value: dce:creator "Dominik Martinát" xsd:string
property_value: dce:date "2024-12-08T15:48:52Z" xsd:dateTime

[Term]
id: MEMON:0000003
name: chemical membrane model
def: "An experimental membrane model that is prepared from non-lipid chemicals that mimic lipid behavior." []
comment: For example, 1-octanol in water is commonly used to predict the partition coefficient of molecules between hydrophilic and lipophilic environments.
is_a: MEMON:0000001 ! experimental membrane model
property_value: dce:creator "Dominik Martinát" xsd:string
property_value: dce:date "2024-12-08T15:52:08Z" xsd:dateTime

[Term]
id: MEMON:0000004
name: membrane model component
def: "A molecular component from which a membrane model consists." []
is_a: BFO:0000004
relationship: RO:0002180 MEMON:0000004 ! membrane model component
property_value: dce:creator "Dominik Martinát" xsd:string
property_value: dce:date "2024-12-08T15:53:09Z" xsd:dateTime

[Term]
id: MEMON:0000005
name: computational membrane model
def: "A membrane model that is used in computational predictions of membrane properties." []
is_a: MEMON:0000008 ! membrane model
property_value: dce:creator "Dominik Martinát" xsd:string
property_value: dce:date "2024-12-08T15:57:54Z" xsd:dateTime

[Term]
id: MEMON:0000006
name: QSAR membrane model
def: "A computational membrane model that is utilized for Quantitative Structure–Activity Relationship (QSAR) prediction." []
is_a: MEMON:0000005 ! computational membrane model
property_value: dce:creator "Dominik Martinát" xsd:string
property_value: dce:date "2024-12-08T15:58:23Z" xsd:dateTime

[Term]
id: MEMON:0000007
name: simulated membrane
def: "Computational membrane model that is used in membrane simulations." []
comment: For example, a lipid bilayer assembled for molecular dynamics simulation.
is_a: MEMON:0000005 ! computational membrane model
property_value: dce:creator "Dominik Martinát" xsd:string
property_value: dce:date "2024-12-08T15:58:59Z" xsd:dateTime

[Term]
id: MEMON:0000008
name: membrane model
def: "A scientific model that is used to predict the properties of biological membranes." []
is_a: BFO:0000004
property_value: dce:creator "Dominik Martinát" xsd:string
property_value: dce:date "2024-12-08T16:21:07Z" xsd:dateTime

