format-version: 1.2
data-version: memon/releases/2024-12-12/memon-simple.owl
subsetdef: ro-eco ""
idspace: dc http://purl.org/dc/elements/1.1/ 
idspace: oboInOwl http://www.geneontology.org/formats/oboInOwl# 
idspace: terms http://purl.org/dc/terms/ 
ontology: memon/memon-simple
property_value: owl:versionInfo "2024-12-12" xsd:string
property_value: terms:description "An ontology about cell membranes and their models" xsd:string
property_value: terms:license https://creativecommons.org/publicdomain/zero/1.0/
property_value: terms:title "Membrane Ontology" xsd:string

[Term]
id: MEMON:0000001
name: experimental membrane model
def: "A membrane model that is used in experiments." []
is_a: MEMON:0000008 ! membrane model
relationship: RO:0002180 MEMON:0000004 ! has component membrane model component
property_value: dc:creator "Dominik Martinát" xsd:string
property_value: dc:date "2024-12-08T15:48:12Z" xsd:dateTime

[Term]
id: MEMON:0000002
name: artificial lipid membrane
def: "An experimental membrane model that is prepared from lipids." []
comment: For example membrane consisting of DOPC.
is_a: MEMON:0000001 ! experimental membrane model
property_value: dc:creator "Dominik Martinát" xsd:string
property_value: dc:date "2024-12-08T15:48:52Z" xsd:dateTime

[Term]
id: MEMON:0000003
name: chemical membrane model
def: "An experimental membrane model that is prepared from non-lipid chemicals that mimic lipid behavior." []
comment: For example, 1-octanol in water is commonly used to predict the partition coefficient of molecules between hydrophilic and lipophilic environments.
is_a: MEMON:0000001 ! experimental membrane model
property_value: dc:creator "Dominik Martinát" xsd:string
property_value: dc:date "2024-12-08T15:52:08Z" xsd:dateTime

[Term]
id: MEMON:0000004
name: membrane model component
def: "A molecular component from which a membrane model consists." []
relationship: RO:0002180 MEMON:0000004 ! has component membrane model component
property_value: dc:creator "Dominik Martinát" xsd:string
property_value: dc:date "2024-12-08T15:53:09Z" xsd:dateTime

[Term]
id: MEMON:0000005
name: computational membrane model
def: "A membrane model that is used in computational predictions of membrane properties." []
is_a: MEMON:0000008 ! membrane model
property_value: dc:creator "Dominik Martinát" xsd:string
property_value: dc:date "2024-12-08T15:57:54Z" xsd:dateTime

[Term]
id: MEMON:0000006
name: QSAR membrane model
def: "A computational membrane model that is utilized for Quantitative Structure–Activity Relationship (QSAR) prediction." []
is_a: MEMON:0000005 ! computational membrane model
property_value: dc:creator "Dominik Martinát" xsd:string
property_value: dc:date "2024-12-08T15:58:23Z" xsd:dateTime

[Term]
id: MEMON:0000007
name: simulated membrane
def: "Computational membrane model that is used in membrane simulations." []
comment: For example, a lipid bilayer assembled for molecular dynamics simulation.
is_a: MEMON:0000005 ! computational membrane model
property_value: dc:creator "Dominik Martinát" xsd:string
property_value: dc:date "2024-12-08T15:58:59Z" xsd:dateTime

[Term]
id: MEMON:0000008
name: membrane model
def: "A scientific model that is used to predict the properties of biological membranes." []
property_value: dc:creator "Dominik Martinát" xsd:string
property_value: dc:date "2024-12-08T16:21:07Z" xsd:dateTime

[Typedef]
id: RO:0002180
name: has component
def: "w 'has component' p if w 'has part' p and w is such that it can be directly disassembled into into n parts p, p2, p3, ..., pn, where these parts are of similar type." []
subset: ro-eco
property_value: IAO:0000114 IAO:0000125
property_value: IAO:0000116 "The definition of 'has component' is still under discussion. The challenge is in providing a definition that does not imply transitivity." xsd:string
property_value: IAO:0000232 "For use in recording has_part with a cardinality constraint, because OWL does not permit cardinality constraints to be used in combination with transitive object properties. In situations where you would want to say something like 'has part exactly 5 digit, you would instead use has_component exactly 5 digit." xsd:string
property_value: RO:0001900 RO:0001901
property_value: seeAlso http://ontologydesignpatterns.org/wiki/Submissions:Componency

